Timing cleanup

timing/examples/FreeRTOS_tasks_noasserts_proofs_clz.v
@@ -3,88 +3,64 @@ Require Import riscvTiming.
 Import RISCVNotations.
 Require Import memsolve.
 
-Definition start_vTaskSwitchContext : N := 0x8000137c.
-Definition end_vTaskSwitchContext : N := 0x8000144c.
-
+(* Some machinery describing the CPU *)
 Variable ML : N.
 Variable ML_pos : 1 <= ML.
-
 Module riscv_toa.
     Definition time_of_addr (s : store) (a : addr) : N :=
         match neorv32_cycles_upper_bound ML s (RTOSDemo_NoAsserts_Clz a) with
         | Some x => x | _ => 0 end.
 End riscv_toa.
-
 Module riscvT := MakeTimingContents riscvTiming riscv_toa.
 Export riscvT.
-
 Definition cycle_count_of_trace := cycle_count_of_trace time_of_addr.
 
+(* These expressions pop up a lot and I don't like seeing them, so just fold them up
+   - time_mem    = The time in clock cycles of a memory access
+   - time_branch = The time in clock cycles of a successful/taken branch
+*)
 Definition time_mem : N :=
     5 + (ML - 2).
-
 Definition time_branch : N :=
     5 + (ML - 1).
 
+(* The doubleword in static memory (offset of gp) that determines if the scheduler
+   is suspended. The scheduler should be suspended when any critical behavior
+   is ongoing that could be disrupted by context switching
+   - Memory allocation
+   - Atomic operations
+   - Modifying shared memory
+   - Performance optimization
+*)
 Definition uxSchedulerSuspended (gp : N) (mem : addr -> N) : N :=
-    (* mem Ⓓ[2144 + gp]. *)
-    (* This should actually be the below expression. Unclear on whether lifter
-       has bug, seems like it isn't treating immediate as signed
-    *)
     mem Ⓓ[gp ⊖ 1952].
 
-Definition addr_xYieldPendings (gp : N) : N :=
+(* The address of the doubleword in static memory that is nonzero when a task is
+   ready to "yield," or signal that a context switch needs to occur (either 
+   voluntarily or involuntarily)
+*)
+Definition addr_xYieldPendings (gp : N) : addr :=
     gp - 1932.
 
+(* A pointer in static memory to the Current Task Control Block (TCB). The TCB
+   is a data structure containing all essential information for managing a task.
+*)
 Definition pxCurrentTCB (gp : N) (mem : addr -> N) : N :=
-    (* mem Ⓓ[2200 + gp]. *)
-    (* Same as above *)
     mem Ⓓ[gp ⊖ 1896].
 
+(* The doubleword in static memory that records the highest priority out of all
+   currently-ready tasks.
+*)
 Definition uxTopReadyPriority (gp : N) (mem : addr -> N) : N :=
     mem Ⓓ[gp ⊖ 1920].
 
-Definition addr_pxReadyTasksLists (gp : N) : N :=
+(* The address in static memory of a list of linked-lists that record all currently-
+   ready tasks. The index into pxReadyTasksLists indicates those tasks' priority.
+*)
+Definition addr_pxReadyTasksLists (gp : N) : addr :=
     gp ⊖ 924.
 
-Definition vTaskSwitchContext_exit (t:trace) :=
-  match t with (Addr a,_)::_ => match a with
-  | 0x8000138c | 0x8000144c => true
-  | _ => false
-  end | _ => false end.
-
-Definition __global_pointer : N := 0x80080800.
-Definition __global_size : N := 2048.
-Definition __stack_pointer : N :=
-    (* Section 4.4.2. RAM Layout - 
-        The stack starts at the very end of the RAM at address ORIGIN(ram) + LENGTH(ram) - 4.
-        The stack grows downwards.*)
-    (* https://cdn.hackaday.io/files/1741677451560928/NEORV32.pdf *)
-    (2 ^ 32) - 4.
-
-Definition vTaskSwitchContext_stack_frame_size : N := 16.
-
-Definition gp_sp_noverlap (gp sp : N) : Prop :=
-    ~overlap 32 (gp ⊖ __global_size) __global_size (sp ⊖ vTaskSwitchContext_stack_frame_size) vTaskSwitchContext_stack_frame_size.
-
-Fixpoint subtrace_since_address (t : trace) (a : addr) : trace :=
-    match t with
-    | (Addr a', st) :: tl => if (a =? a') then (Addr a', st) :: nil else
-        (Addr a', st) :: subtrace_since_address tl a
-    | _ => nil
-    end.
-
-Fixpoint subtrace_before_address (t : trace) (a : addr) : trace :=
-    match t with
-    | (Addr a', st) :: tl => if (a =? a') then tl else
-        subtrace_before_address tl a
-    | _ => nil
-    end.
-
-Definition time_before_address (t : trace) (a : addr) :=
-    cycle_count_of_trace (subtrace_before_address t a).
-
-(* The goal with the above function is to use for function timing invariants, e.g.
+(* The goal with the below functions is to use for function timing invariants, e.g.
         cycle_count_of_trace t' = 
             func_time + cycle_count_of_trace (subtrace_before_address t' func_entry_addr))
     This would be nice because then you don't have to worry about annoying arithmetic.
@@ -105,6 +81,39 @@ Definition time_before_address (t : trace) (a : addr) :=
     Will have to revisit later, definitely need something like this for scaling up.
 *)
 
+Fixpoint subtrace_since_address (t : trace) (a : addr) : trace :=
+    match t with
+    | (Addr a', st) :: tl => if (a =? a') then (Addr a', st) :: nil else
+        (Addr a', st) :: subtrace_since_address tl a
+    | _ => nil
+    end.
+
+Fixpoint subtrace_before_address (t : trace) (a : addr) : trace :=
+    match t with
+    | (Addr a', st) :: tl => if (a =? a') then tl else
+        subtrace_before_address tl a
+    | _ => nil
+    end.
+
+Definition time_before_address (t : trace) (a : addr) : N :=
+    cycle_count_of_trace (subtrace_before_address t a).
+
+(* The size of static memory (at the bottom of memory) and stack memory (at the
+   top)
+*)
+Definition __global_size : N := 2048.
+Definition vTaskSwitchContext_stack_frame_size : N := 16.
+
+(* What follows are a list of assumptions we make about the well-formedness of
+   static and stack memory. For example: static and stack memory should not overlap
+   (this would be a stack overflow)
+*)
+Definition gp_sp_noverlap (gp sp : N) : Prop :=
+    ~overlap 32 (gp ⊖ __global_size) __global_size (sp ⊖ vTaskSwitchContext_stack_frame_size) vTaskSwitchContext_stack_frame_size.
+
+(* These two definitions state that any two of the above buffers we're interested
+   in do not overlap
+*)
 Definition static_buffer_lengths_in_bytes (a : addr) : option N :=
     match a with
     (* uxSchedulerSuspended *)
@@ -115,7 +124,6 @@ Definition static_buffer_lengths_in_bytes (a : addr) : option N :=
     | 1896 
     (* uxTopReadyPriority *)
     | 1920 => Some 4
-    (* TODO : Prove that smem_well_formed doesn't break with this in it *)
     | _ => None
     end.
 
@@ -128,77 +136,93 @@ Definition smem_well_formed (gp : N) : Prop :=
                 (gp ⊖ x) len_x
                 (gp ⊖ y) len_y.
 
-Definition pxCurrentTCB_noverlap_clz_static (gp : N) mem : Prop :=
+(* I don't yet know the significance of the address
+      gp ⊖ 920 ⊕ (31 ⊖ clz (uxTopReadyPriority gp mem) 32) * 20
+   but it appears very frequently and it must not overlap with things like the
+   TCB or stack memory. Some of these assumptions can actually be proven due to 
+   the boundaries of clz (count leading zeroes) being 0..32
+*)
+Definition pxCurrentTCB_noverlap_clz_static (gp : N) (mem : addr -> N) : Prop :=
     ~ overlap 32
         (48 + pxCurrentTCB gp mem) 4
-        (gp ⊖ 920 ⊕ (31 ⊖ clz (mem Ⓓ[ gp ⊖ 1920 ]) 32) * 20) 4.
+        (gp ⊖ 920 ⊕ (31 ⊖ clz (uxTopReadyPriority gp mem) 32) * 20) 4.
 
 Definition clz_noverlap_smem (gp : N) mem : Prop :=
     forall x len_x,
         static_buffer_lengths_in_bytes x = Some len_x ->
         ~ overlap 32
             (gp ⊖ x) len_x
-            (gp ⊖ 920 ⊕ (31 ⊖ clz (mem Ⓓ[ gp ⊖ 1920 ]) 32) * 20) 4.
+            (gp ⊖ 920 ⊕ (31 ⊖ clz (uxTopReadyPriority gp mem) 32) * 20) 4.
 
-Definition pxCurrentTCB_noverlap_static (gp : N) mem : Prop :=
+(* The TCB doesn't overlap static memory or the stack frame *)
+Definition pxCurrentTCB_noverlap_static (gp : N) (mem : addr -> N) : Prop :=
     forall x len_x,
         static_buffer_lengths_in_bytes x = Some len_x ->
         ~ overlap 32
             (48 + pxCurrentTCB gp mem) 4
             (gp ⊖ x) len_x.
 
-Definition pxCurrentTCB_noverlap_stackframe (gp base_sp : N) mem : Prop :=
+Definition pxCurrentTCB_noverlap_stackframe (gp base_sp : N) (mem : addr -> N) : Prop :=
     ~ overlap 32
         (48 + pxCurrentTCB gp mem) 4
         (base_sp ⊖ 16) 16.
 
-Definition mem_pxCurrentTCB_noverlap_stackframe (gp base_sp : N) mem : Prop :=
+(* The address contained in the current TCB doesn't overlap with static memory
+   or the stack frame *)
+Definition mem_pxCurrentTCB_noverlap_stackframe (gp base_sp : N) (mem : addr -> N) : Prop :=
     ~ overlap 32
         (mem Ⓓ[48 + pxCurrentTCB gp mem]) 4
         (base_sp ⊖ 16) 16.
 
-Definition mem_pxCurrentTCB_noverlap_static (gp : N) mem : Prop :=
+Definition mem_pxCurrentTCB_noverlap_static (gp : N) (mem : addr -> N) : Prop :=
     forall x len_x,
         static_buffer_lengths_in_bytes x = Some len_x ->
         ~ overlap 32
             (mem Ⓓ[48 + pxCurrentTCB gp mem]) 4
             (gp ⊖ x) len_x.
 
-Definition offset_mem_pxCurrentTCB_noverlap_clz (gp : N) mem : Prop :=
+(* Offsets into the address contained in the current TCB don't overlap with 
+   the clz address or stack memory *)
+Definition offset_mem_pxCurrentTCB_noverlap_clz (gp : N) (mem : addr -> N) : Prop :=
     forall k, k = 8 \/ k = 12 ->
         ~ overlap 32
             (k + mem Ⓓ[48 + pxCurrentTCB gp mem]) 4
-            (gp ⊖ 920 ⊕ (31 ⊖ clz (mem Ⓓ[ gp ⊖ 1920 ]) 32) * 20) 4.
+            (gp ⊖ 920 ⊕ (31 ⊖ clz (uxTopReadyPriority gp mem) 32) * 20) 4.
 
-Definition clz_noverlap_sframe (gp base_sp : N) mem : Prop :=
+Definition clz_noverlap_sframe (gp base_sp : N) (mem : addr -> N) : Prop :=
     ~ overlap 32 
         (base_sp ⊖ 16) 16
-        (gp ⊖ 920 ⊕ (31 ⊖ clz (mem Ⓓ[ gp ⊖ 1920 ]) 32) * 20) 4.
+        (gp ⊖ 920 ⊕ (31 ⊖ clz (uxTopReadyPriority gp mem) 32) * 20) 4.
 
-Definition mem4_pxCurrentTCB_noverlap_stackframe gp base_sp mem :=
+(* An offset into the buffer at the clz address doesn't overlap with static
+   memory or the stack frame *)
+Definition mem4_pxCurrentTCB_noverlap_stackframe (gp base_sp : N) (mem : addr -> N) : Prop :=
         ~ overlap 32
         (base_sp ⊖ 16) 16
-            (4 + mem Ⓓ[gp ⊖ 920 ⊕ (31 ⊖ clz (mem Ⓓ[ gp ⊖ 1920 ]) 32) * 20]) 4.
+            (4 + mem Ⓓ[gp ⊖ 920 ⊕ (31 ⊖ clz (uxTopReadyPriority gp mem) 32) * 20]) 4.
 
-Definition mem4_pxCurrentTCB_noverlap_static gp mem :=
+Definition mem4_pxCurrentTCB_noverlap_static (gp : N) (mem : addr -> N) : Prop :=
     forall x len_x,
         static_buffer_lengths_in_bytes x = Some len_x ->
         ~ overlap 32
             (gp ⊖ x) 4
-            (4 + mem Ⓓ[gp ⊖ 920 ⊕ (31 ⊖ clz (mem Ⓓ[ gp ⊖ 1920 ]) 32) * 20]) 4.
+            (4 + mem Ⓓ[gp ⊖ 920 ⊕ (31 ⊖ clz (uxTopReadyPriority gp mem) 32) * 20]) 4.
 
-Definition mem4_mem4_noverlap_stackframe gp base_sp mem :=
+(* An offset into the buffer at an offset into the buffer at the clz address 
+   doesn't overlap with static memory or the stack frame *)
+Definition mem4_mem4_noverlap_stackframe (gp base_sp : N) (mem : addr -> N) :=
     ~ overlap 32
         (base_sp ⊖ 16) 16
-        (4 + mem Ⓓ[ 4 + mem Ⓓ[ gp ⊖ 920 ⊕ (31 ⊖ clz (mem Ⓓ[ gp ⊖ 1920 ]) 32) * 20 ] ]) 4.
+        (4 + mem Ⓓ[ 4 + mem Ⓓ[ gp ⊖ 920 ⊕ (31 ⊖ clz (uxTopReadyPriority gp mem) 32) * 20 ] ]) 4.
 
-Definition mem4_mem4_noverlap_static gp mem :=
+Definition mem4_mem4_noverlap_static (gp : N) (mem : addr -> N) :=
     forall x len_x,
         static_buffer_lengths_in_bytes x = Some len_x ->
         ~ overlap 32
             (gp ⊖ x) 4
-            (4 + mem Ⓓ[ 4 + mem Ⓓ[ gp ⊖ 920 ⊕ (31 ⊖ clz (mem Ⓓ[ gp ⊖ 1920 ]) 32) * 20 ] ]) 4.
+            (4 + mem Ⓓ[ 4 + mem Ⓓ[ gp ⊖ 920 ⊕ (31 ⊖ clz (uxTopReadyPriority gp mem) 32) * 20 ] ]) 4.
 
+(* Stick them all together *)
 Definition common_noverlaps gp base_sp mem : Prop :=
     gp_sp_noverlap gp base_sp /\
     smem_well_formed gp /\
@@ -213,19 +237,31 @@ Definition common_noverlaps gp base_sp mem : Prop :=
     mem4_pxCurrentTCB_noverlap_stackframe gp base_sp mem /\
     mem4_pxCurrentTCB_noverlap_static gp mem.
 
-(* TODO : Rewrite postconditions, the if conditions are garbage from earlier versions *)
-Definition timing_postcondition (t : trace) (gp : N) (mem : addr -> N) : Prop :=
+Definition time_of_vTaskSwitchContext (t : trace) (gp : N) (mem : addr -> N) : Prop :=
+    (* is the scheduler suspended *)
     if (uxSchedulerSuspended gp mem) =? 0 then
-        cycle_count_of_trace t = 25 + 3 * time_branch + 17 * time_mem
-        + (if (mem Ⓓ[ 4 + mem Ⓓ[ gp ⊖ 920 ⊕ (31 ⊖ clz (uxTopReadyPriority gp mem) 32) * 20 ] ])
-            =? ((gp ⊖ 916) ⊕ (31 ⊖ clz (uxTopReadyPriority gp mem) 32) * 20)
-            then 22 + clz (mem Ⓓ[ 4294965376 + gp ]) 32 + 5 * time_mem else
-            19 + time_branch + clz (mem Ⓓ[ 4294965376 + gp ]) 32 + 3 * time_mem
-        )
+        cycle_count_of_trace t = (* total number of cycles equals... *)
+        25 + 3 * time_branch + 17 * time_mem
+            (* This branch condition isn't well-documented, need to dig into source *)
+          + (if (mem Ⓓ[ 4 + mem Ⓓ[ gp ⊖ 920 ⊕ (31 ⊖ clz (uxTopReadyPriority gp mem) 32) * 20 ] ])
+              =? ((gp ⊖ 916) ⊕ (31 ⊖ clz (uxTopReadyPriority gp mem) 32) * 20)
+              then 
+                22 + (clz (uxTopReadyPriority gp mem) 32) + 5 * time_mem 
+              else
+                19 + time_branch + (clz (uxTopReadyPriority gp mem) 32) + 3 * time_mem
+              (* time_branch = 5 + (memory latency - 1), # of cycles for a successful/taken branch *)
+              (* time_mem = 5 + (memory latency - 2), # of cycles for a memory retreival *)
+          )
     else
         cycle_count_of_trace t = 5 + time_branch + 2 * time_mem.
 
-Definition vTaskSwitchContext_timing_invs (_ : store) (p : addr) (base_sp gp : N) (base_mem : addr -> N) (t:trace) :=
+(* The invariant set for the proof. These are waypoints that guide us towards 
+   the postcondition. We state properties here that we want to remember for later
+   in the proof (anything not in an invariant is forgotten after a branch).
+   The properties that we state help us prove the postcondition. We must prove
+   each invariant throughout the proof. *)
+Definition vTaskSwitchContext_timing_invs (_ : store) (p : addr) 
+    (base_sp gp : N) (base_mem : addr -> N) (t:trace) : option Prop :=
 match t with (Addr a, s) :: t' => match a with
     (* vApplicationStackOverflowHook *)
     (* NOTE : This function intentionally goes into an infinite loop when a
@@ -241,196 +277,137 @@ match t with (Addr a, s) :: t' => match a with
             mem4_mem4_noverlap_stackframe gp base_sp mem /\
             mem4_mem4_noverlap_static gp mem /\
             ~ overlap 32
-                (gp ⊖ 920 ⊕ (31 ⊖ clz (mem Ⓓ[ gp ⊖ 1920 ]) 32) * 20) 4
-                (4 + mem Ⓓ[ gp ⊖ 920 ⊕ (31 ⊖ clz (mem Ⓓ[ gp ⊖ 1920 ]) 32) * 20 ] ) 4 /\
+                (gp ⊖ 920 ⊕ (31 ⊖ clz (uxTopReadyPriority gp mem) 32) * 20) 4
+                (4 + mem Ⓓ[ gp ⊖ 920 ⊕ (31 ⊖ clz (uxTopReadyPriority gp mem) 32) * 20 ] ) 4 /\
             ~ overlap 32
-                (gp ⊖ 920 ⊕ (31 ⊖ clz (mem Ⓓ[ gp ⊖ 1920 ]) 32) * 20) 4
-                (mem Ⓓ[4 + mem Ⓓ[ gp ⊖ 920 ⊕ (31 ⊖ clz (mem Ⓓ[ gp ⊖ 1920 ]) 32) * 20 ]]) 4 /\
+                (gp ⊖ 920 ⊕ (31 ⊖ clz (uxTopReadyPriority gp mem) 32) * 20) 4
+                (mem Ⓓ[4 + mem Ⓓ[ gp ⊖ 920 ⊕ (31 ⊖ clz (uxTopReadyPriority gp mem) 32) * 20 ]]) 4 /\
             uxTopReadyPriority gp mem = uxTopReadyPriority gp base_mem /\
-            mem Ⓓ[ 4 + mem Ⓓ[ gp ⊖ 920 + (31 ⊖ clz (mem Ⓓ[ gp ⊖ 1920 ]) 32) * 20 ] ] =
-            base_mem Ⓓ[ 4 + base_mem Ⓓ[ gp ⊖ 920 + (31 ⊖ clz (base_mem Ⓓ[ gp ⊖ 1920 ]) 32) * 20 ] ]  /\
+            mem Ⓓ[ 4 + mem Ⓓ[ gp ⊖ 920 + (31 ⊖ clz (uxTopReadyPriority gp mem) 32) * 20 ] ] =
+            base_mem Ⓓ[ 4 + base_mem Ⓓ[ gp ⊖ 920 + (31 ⊖ clz (uxTopReadyPriority gp base_mem) 32) * 20 ] ]  /\
         cycle_count_of_trace t' = time_mem)
     | 0x800013b4 => Some (exists mem, s V_MEM32 = Ⓜmem /\ 
-        s R_GP = Ⓓgp /\ s R_SP = Ⓓ(base_sp ⊖ 16) /\
-        s R_A5 = Ⓓ(mem Ⓓ[48 + pxCurrentTCB gp mem]) /\
-        s R_A2 = Ⓓ(mem Ⓓ[mem Ⓓ[48 + pxCurrentTCB gp mem]]) /\
-        s R_A4 = Ⓓ((0xa5a5a << 12) + 1445) /\
+        s R_GP = Ⓓgp /\
         common_noverlaps gp base_sp mem /\
         mem4_mem4_noverlap_stackframe gp base_sp mem /\
         mem4_mem4_noverlap_static gp mem /\
         ~ overlap 32
-            (gp ⊖ 920 ⊕ (31 ⊖ clz (mem Ⓓ[ gp ⊖ 1920 ]) 32) * 20) 4
-            (4 + mem Ⓓ[ gp ⊖ 920 ⊕ (31 ⊖ clz (mem Ⓓ[ gp ⊖ 1920 ]) 32) * 20 ] ) 4 /\
+            (gp ⊖ 920 ⊕ (31 ⊖ clz (uxTopReadyPriority gp mem) 32) * 20) 4
+            (4 + mem Ⓓ[ gp ⊖ 920 ⊕ (31 ⊖ clz (uxTopReadyPriority gp mem) 32) * 20 ] ) 4 /\
         ~ overlap 32
-            (gp ⊖ 920 ⊕ (31 ⊖ clz (mem Ⓓ[ gp ⊖ 1920 ]) 32) * 20) 4
-            (mem Ⓓ[4 + mem Ⓓ[ gp ⊖ 920 ⊕ (31 ⊖ clz (mem Ⓓ[ gp ⊖ 1920 ]) 32) * 20 ]]) 4 /\
+            (gp ⊖ 920 ⊕ (31 ⊖ clz (uxTopReadyPriority gp mem) 32) * 20) 4
+            (mem Ⓓ[4 + mem Ⓓ[ gp ⊖ 920 ⊕ (31 ⊖ clz (uxTopReadyPriority gp mem) 32) * 20 ]]) 4 /\
         uxTopReadyPriority gp mem = uxTopReadyPriority gp base_mem /\
-        mem Ⓓ[ 4 + mem Ⓓ[ gp ⊖ 920 + (31 ⊖ clz (mem Ⓓ[ gp ⊖ 1920 ]) 32) * 20 ] ] =
-        base_mem Ⓓ[ 4 + base_mem Ⓓ[ gp ⊖ 920 + (31 ⊖ clz (base_mem Ⓓ[ gp ⊖ 1920 ]) 32) * 20 ] ]  /\
+        mem Ⓓ[ 4 + mem Ⓓ[ gp ⊖ 920 + (31 ⊖ clz (uxTopReadyPriority gp mem) 32) * 20 ] ] =
+            base_mem Ⓓ[ 4 + base_mem Ⓓ[ gp ⊖ 920 + (31 ⊖ clz (uxTopReadyPriority gp base_mem) 32) * 20 ] ]  /\
         (uxSchedulerSuspended gp base_mem =? 0) = true /\
         cycle_count_of_trace t' = 6 + 7 * time_mem + time_branch)
     | 0x800013bc => Some (exists mem, s V_MEM32 = Ⓜmem /\ 
-        s R_GP = Ⓓgp /\ s R_SP = Ⓓ(base_sp ⊖ 16) /\
-        s R_A2 = Ⓓ(mem Ⓓ[mem Ⓓ[48 + pxCurrentTCB gp mem]]) /\
-        s R_A3 = Ⓓ(mem Ⓓ[4 + mem Ⓓ[48 + pxCurrentTCB gp mem]]) /\
-        s R_A5 = Ⓓ(mem Ⓓ[48 + pxCurrentTCB gp mem]) /\
+        s R_GP = Ⓓgp /\
         common_noverlaps gp base_sp mem /\
         mem4_mem4_noverlap_stackframe gp base_sp mem /\
         mem4_mem4_noverlap_static gp mem /\
         ~ overlap 32
-            (gp ⊖ 920 ⊕ (31 ⊖ clz (mem Ⓓ[ gp ⊖ 1920 ]) 32) * 20) 4
-            (4 + mem Ⓓ[ gp ⊖ 920 ⊕ (31 ⊖ clz (mem Ⓓ[ gp ⊖ 1920 ]) 32) * 20 ] ) 4 /\
+            (gp ⊖ 920 ⊕ (31 ⊖ clz (uxTopReadyPriority gp mem) 32) * 20) 4
+            (4 + mem Ⓓ[ gp ⊖ 920 ⊕ (31 ⊖ clz (uxTopReadyPriority gp mem) 32) * 20 ] ) 4 /\
         ~ overlap 32
-            (gp ⊖ 920 ⊕ (31 ⊖ clz (mem Ⓓ[ gp ⊖ 1920 ]) 32) * 20) 4
-            (mem Ⓓ[4 + mem Ⓓ[ gp ⊖ 920 ⊕ (31 ⊖ clz (mem Ⓓ[ gp ⊖ 1920 ]) 32) * 20 ]]) 4 /\
+            (gp ⊖ 920 ⊕ (31 ⊖ clz (uxTopReadyPriority gp mem) 32) * 20) 4
+            (mem Ⓓ[4 + mem Ⓓ[ gp ⊖ 920 ⊕ (31 ⊖ clz (uxTopReadyPriority gp mem) 32) * 20 ]]) 4 /\
         uxTopReadyPriority gp mem = uxTopReadyPriority gp base_mem /\
-        mem Ⓓ[ 4 + mem Ⓓ[ gp ⊖ 920 + (31 ⊖ clz (mem Ⓓ[ gp ⊖ 1920 ]) 32) * 20 ] ] =
-        base_mem Ⓓ[ 4 + base_mem Ⓓ[ gp ⊖ 920 + (31 ⊖ clz (base_mem Ⓓ[ gp ⊖ 1920 ]) 32) * 20 ] ]  /\
+        mem Ⓓ[ 4 + mem Ⓓ[ gp ⊖ 920 + (31 ⊖ clz (uxTopReadyPriority gp mem) 32) * 20 ] ] =
+            base_mem Ⓓ[ 4 + base_mem Ⓓ[ gp ⊖ 920 + (31 ⊖ clz (uxTopReadyPriority gp base_mem) 32) * 20 ] ]  /\
         (uxSchedulerSuspended gp base_mem =? 0) = true /\
-        (mem Ⓓ[ mem Ⓓ[ 48 + pxCurrentTCB gp mem ] ] =? 0xa5a5a5a5) = true /\
         cycle_count_of_trace t' = 9 + 8 * time_mem + time_branch)
     | 0x800013c4 => Some (exists mem, s V_MEM32 = Ⓜmem /\ 
-        s R_GP = Ⓓgp /\ s R_SP = Ⓓ(base_sp ⊖ 16) /\
-        s R_A3 = Ⓓ(mem Ⓓ[4 + mem Ⓓ[48 + pxCurrentTCB gp mem]]) /\
-        s R_A4 = Ⓓ(mem Ⓓ[8 + mem Ⓓ[48 + pxCurrentTCB gp mem]]) /\
-        s R_A5 = Ⓓ(mem Ⓓ[48 + pxCurrentTCB gp mem]) /\
+        s R_GP = Ⓓgp /\
         common_noverlaps gp base_sp mem /\
         mem4_mem4_noverlap_stackframe gp base_sp mem /\
         mem4_mem4_noverlap_static gp mem /\
         ~ overlap 32
-            (gp ⊖ 920 ⊕ (31 ⊖ clz (mem Ⓓ[ gp ⊖ 1920 ]) 32) * 20) 4
-            (4 + mem Ⓓ[ gp ⊖ 920 ⊕ (31 ⊖ clz (mem Ⓓ[ gp ⊖ 1920 ]) 32) * 20 ] ) 4 /\
+            (gp ⊖ 920 ⊕ (31 ⊖ clz (uxTopReadyPriority gp mem) 32) * 20) 4
+            (4 + mem Ⓓ[ gp ⊖ 920 ⊕ (31 ⊖ clz (uxTopReadyPriority gp mem) 32) * 20 ] ) 4 /\
         ~ overlap 32
-            (gp ⊖ 920 ⊕ (31 ⊖ clz (mem Ⓓ[ gp ⊖ 1920 ]) 32) * 20) 4
-            (mem Ⓓ[4 + mem Ⓓ[ gp ⊖ 920 ⊕ (31 ⊖ clz (mem Ⓓ[ gp ⊖ 1920 ]) 32) * 20 ]]) 4 /\
+            (gp ⊖ 920 ⊕ (31 ⊖ clz (uxTopReadyPriority gp mem) 32) * 20) 4
+            (mem Ⓓ[4 + mem Ⓓ[ gp ⊖ 920 ⊕ (31 ⊖ clz (uxTopReadyPriority gp mem) 32) * 20 ]]) 4 /\
         uxTopReadyPriority gp mem = uxTopReadyPriority gp base_mem /\
-        mem Ⓓ[ 4 + mem Ⓓ[ gp ⊖ 920 + (31 ⊖ clz (mem Ⓓ[ gp ⊖ 1920 ]) 32) * 20 ] ] =
-        base_mem Ⓓ[ 4 + base_mem Ⓓ[ gp ⊖ 920 + (31 ⊖ clz (base_mem Ⓓ[ gp ⊖ 1920 ]) 32) * 20 ] ]  /\
-        (mem Ⓓ[ mem Ⓓ[ 48 + pxCurrentTCB gp mem ] ] =? 0xa5a5a5a5) = true /\
-        (mem Ⓓ[4 + mem Ⓓ[48 + pxCurrentTCB gp mem]] =? mem Ⓓ[mem Ⓓ[48 + pxCurrentTCB gp mem]]) = true /\
+        mem Ⓓ[ 4 + mem Ⓓ[ gp ⊖ 920 + (31 ⊖ clz (uxTopReadyPriority gp mem) 32) * 20 ] ] =
+            base_mem Ⓓ[ 4 + base_mem Ⓓ[ gp ⊖ 920 + (31 ⊖ clz (uxTopReadyPriority gp base_mem) 32) * 20 ] ]  /\
         (uxSchedulerSuspended gp base_mem =? 0) = true /\
         cycle_count_of_trace t' = 12 + 9 * time_mem + time_branch
     )
     | 0x800013cc => Some (exists mem, s V_MEM32 = Ⓜmem /\ 
-        s R_GP = Ⓓgp /\ s R_SP = Ⓓ(base_sp ⊖ 16) /\
-        s R_A3 = Ⓓ(mem Ⓓ[4 + mem Ⓓ[48 + pxCurrentTCB gp mem]]) /\
-        s R_A4 = Ⓓ(mem Ⓓ[8 + mem Ⓓ[48 + pxCurrentTCB gp mem]]) /\
-        s R_A5 = Ⓓ(mem Ⓓ[12 + mem Ⓓ[48 + pxCurrentTCB gp mem]]) /\
+        s R_GP = Ⓓgp /\
         common_noverlaps gp base_sp mem /\
         mem4_mem4_noverlap_stackframe gp base_sp mem /\
         mem4_mem4_noverlap_static gp mem /\
         ~ overlap 32
-            (gp ⊖ 920 ⊕ (31 ⊖ clz (mem Ⓓ[ gp ⊖ 1920 ]) 32) * 20) 4
-            (4 + mem Ⓓ[ gp ⊖ 920 ⊕ (31 ⊖ clz (mem Ⓓ[ gp ⊖ 1920 ]) 32) * 20 ] ) 4 /\
+            (gp ⊖ 920 ⊕ (31 ⊖ clz (uxTopReadyPriority gp mem) 32) * 20) 4
+            (4 + mem Ⓓ[ gp ⊖ 920 ⊕ (31 ⊖ clz (uxTopReadyPriority gp mem) 32) * 20 ] ) 4 /\
         ~ overlap 32
-            (gp ⊖ 920 ⊕ (31 ⊖ clz (mem Ⓓ[ gp ⊖ 1920 ]) 32) * 20) 4
-            (mem Ⓓ[4 + mem Ⓓ[ gp ⊖ 920 ⊕ (31 ⊖ clz (mem Ⓓ[ gp ⊖ 1920 ]) 32) * 20 ]]) 4 /\
+            (gp ⊖ 920 ⊕ (31 ⊖ clz (uxTopReadyPriority gp mem) 32) * 20) 4
+            (mem Ⓓ[4 + mem Ⓓ[ gp ⊖ 920 ⊕ (31 ⊖ clz (uxTopReadyPriority gp mem) 32) * 20 ]]) 4 /\
         uxTopReadyPriority gp mem = uxTopReadyPriority gp base_mem /\
-        mem Ⓓ[ 4 + mem Ⓓ[ gp ⊖ 920 + (31 ⊖ clz (mem Ⓓ[ gp ⊖ 1920 ]) 32) * 20 ] ] =
-        base_mem Ⓓ[ 4 + base_mem Ⓓ[ gp ⊖ 920 + (31 ⊖ clz (base_mem Ⓓ[ gp ⊖ 1920 ]) 32) * 20 ] ]  /\
-        (mem Ⓓ[ mem Ⓓ[ 48 + pxCurrentTCB gp mem ] ] =? 0xa5a5a5a5) = true /\
-        (mem Ⓓ[4 + mem Ⓓ[48 + pxCurrentTCB gp mem]] =? mem Ⓓ[mem Ⓓ[48 + pxCurrentTCB gp mem]]) = true /\
-        (mem Ⓓ[8 + mem Ⓓ[48 + pxCurrentTCB gp mem]] =? mem Ⓓ[4 + mem Ⓓ[48 + pxCurrentTCB gp mem]]) = true /\
+        mem Ⓓ[ 4 + mem Ⓓ[ gp ⊖ 920 + (31 ⊖ clz (uxTopReadyPriority gp mem) 32) * 20 ] ] =
+            base_mem Ⓓ[ 4 + base_mem Ⓓ[ gp ⊖ 920 + (31 ⊖ clz (uxTopReadyPriority gp base_mem) 32) * 20 ] ]  /\
         (uxSchedulerSuspended gp base_mem =? 0) = true /\
         cycle_count_of_trace t' = 15 + 10 * time_mem + time_branch
     )
     | 0x80001418 => Some (exists mem, s V_MEM32 = Ⓜmem /\ 
-        s R_GP = Ⓓgp /\ s R_SP = Ⓓ(base_sp ⊖ 16) /\
+        s R_GP = Ⓓgp /\
         s R_A1 = Ⓓ(mem Ⓓ[4 + (gp ⊖ 924) ⊕ ((31 ⊖ (clz (uxTopReadyPriority gp mem) 32)) * 20)]) /\
         s R_A2 = Ⓓ(addr_pxReadyTasksLists gp ⊕ ((31 ⊖ (clz (uxTopReadyPriority gp mem) 32)) * 20)) /\
-        s R_A3 = Ⓓ(31 ⊖ clz (uxTopReadyPriority gp mem) 32) /\
-        s R_A4 = Ⓓ(addr_pxReadyTasksLists gp) /\
         s R_A5 = Ⓓ((gp ⊖ 916) ⊕ (31 ⊖ clz (uxTopReadyPriority gp mem) 32) * 20) /\
         common_noverlaps gp base_sp mem /\
         uxTopReadyPriority gp mem = uxTopReadyPriority gp base_mem /\
-        mem Ⓓ[ gp ⊖ 920 + (31 ⊖ clz (mem Ⓓ[ gp ⊖ 1920 ]) 32) * 20 ] =
-            base_mem Ⓓ[ 4 + base_mem Ⓓ[ gp ⊖ 920 + (31 ⊖ clz (base_mem Ⓓ[ gp ⊖ 1920 ]) 32) * 20 ] ]  /\
+        mem Ⓓ[ gp ⊖ 920 + (31 ⊖ clz (uxTopReadyPriority gp mem) 32) * 20 ] =
+            base_mem Ⓓ[ 4 + base_mem Ⓓ[ gp ⊖ 920 + (31 ⊖ clz (uxTopReadyPriority gp base_mem) 32) * 20 ] ]  /\
         (uxSchedulerSuspended gp base_mem =? 0) = true /\
-        (mem Ⓓ[ 12 + mem Ⓓ[ 48 + pxCurrentTCB gp mem ] ] =?
-            mem Ⓓ[ 8 + mem Ⓓ[ 48 + pxCurrentTCB gp mem ] ]) = true /\
-        cycle_count_of_trace t' = 36 + clz (mem Ⓓ[ 4294965376 + gp ]) 32 + 2 * time_branch + 14 * time_mem)
-    | 0x8000138c => Some (
-        timing_postcondition t gp base_mem)
-    | 0x8000144c => Some (
-        timing_postcondition t gp base_mem)
-    | _ => None end
+        cycle_count_of_trace t' = 36 + clz (uxTopReadyPriority gp mem) 32 + 2 * time_branch + 14 * time_mem)
+    | 0x8000138c | 0x8000144c => Some (time_of_vTaskSwitchContext t gp base_mem)
+    | _ => None
+    end
 | _ => None
 end.
 
+(* The exit points for vTaskSwitchContext *)
+Definition vTaskSwitchContext_exit (t:trace) : bool :=
+  match t with (Addr a,_)::_ => match a with
+  | 0x8000138c | 0x8000144c => true
+  | _ => false
+  end | _ => false end.
+
+(* Lift the code into Picinae IL *)
 Definition lifted_vTaskSwitchContext : program :=
     lift_riscv RTOSDemo_NoAsserts_Clz.
 
+(* Let's build some automation machinery to streamline the proof *)
 Ltac unfold_decompose :=
     cbv [decompose_Btype decompose_Itype decompose_Jtype decompose_Rtype 
         decompose_Stype decompose_Utype mask_bit_section]; cbn [N.land].
 Tactic Notation "unfold_decompose" "in" hyp(H) :=
     cbv [decompose_Btype decompose_Itype decompose_Jtype decompose_Rtype 
         decompose_Stype decompose_Utype mask_bit_section] in H; cbn [N.land] in H.
-
 Ltac unfold_time_of_addr :=
     cbv [time_of_addr neorv32_cycles_upper_bound]; cbn - [setmem getmem].
 Tactic Notation "unfold_time_of_addr" "in" hyp(H) :=
     cbv [time_of_addr neorv32_cycles_upper_bound] in H; cbn - [setmem getmem].
-
 Ltac unfold_cycle_count_list :=
     unfold cycle_count_of_trace; repeat rewrite cycle_count_of_trace_cons, cycle_count_of_trace_single; fold cycle_count_of_trace.
-
 Ltac fold_times :=
     fold time_mem; fold time_branch.
-
 Ltac hammer :=
     unfold_cycle_count_list; unfold_time_of_addr; unfold_decompose; fold_times; psimpl; try lia.
 
+(* We use simpl in a few convenient places: make sure it doesn't go haywire *)
 Arguments N.add _ _ : simpl nomatch.
 Arguments N.mul _ _ : simpl nomatch.
 
-Lemma noverlap_index:
-  forall w a1 len1 a2 len2 index size
-  (NO : ~ overlap w a1 len1 a2 len2)
-  (IN : index + size <= len1),
-  ~ overlap w (a1 + index) size a2 len2.
-Proof.
-  intros.
-  remember (a1 + index) as a1'. apply noverlap_shrink with (a1:=a1) (len1:=len1).
-  rewrite Heqa1'. rewrite add_msub_l.
-  apply N.le_trans with (m:=index+size). rewrite <-N.add_le_mono_r. apply N.Div0.mod_le.
-  assumption.
-  assumption.
-Qed.
-
-Lemma getmem_nbyte_distance:
-  forall w e m a1 a2 n v,
-  msub w a1 a2 > n ->
-  msub w a2 a1 > n ->
-    getmem w e n (setmem w e n m a2 v) a1 = getmem w e n m a1.
-Proof.
-  intros.
-  apply getmem_noverlap.
-  clear - H H0.
-  apply sep_noverlap; try (left; lia || right; lia).
-Qed.
-
-(*
-Define some function f
-- f takes in index into GP 
-- f returns length of buffer that is at mem(gp - index) (or none if malformed)
-Assume in theorem that (forall x y, (assume f x, f y are Some number) 
-    x <> y -> ~ overlap (gp - x) (f x) (gp - y) (f y) )
-Assume (forall x, exists k, f x = Some k -> ~ overlap (gp - x) (f x) (sp (-) 16 16 ))
-Now we can specialize assumption for pxcurrenttcb, uxschedulersuspended etc.
-
-Do we assume that these buffers don't overlap with stack frame?
-*)
-
-Theorem clz_le_w : forall n w,
-    clz n w <= w.
-Proof.
-    destruct n; intros; unfold clz; lia.
-Qed.
+(* The entrypoint to vTaskSwitchContext *)
+Definition start_vTaskSwitchContext : N := 0x8000137c.
 
 Theorem vTaskSwitchContext_timing:
   forall s p t s' x' gp sp mem
-         (ENTRY: startof t (x',s') = (Addr start_vTaskSwitchContext,s)) (* Define the entry point of the function *)
+         (ENTRY: startof t (x',s') = (Addr start_vTaskSwitchContext,s))
          (MDL: models rvtypctx s)
          (GP : s R_GP = Ⓓgp)
          (SP : s R_SP = Ⓓsp)
@@ -440,11 +417,11 @@ Theorem vTaskSwitchContext_timing:
             mem4_mem4_noverlap_stackframe gp sp mem /\
             mem4_mem4_noverlap_static gp mem /\
             ~ overlap 32
-                (gp ⊖ 920 ⊕ (31 ⊖ clz (mem Ⓓ[ gp ⊖ 1920 ]) 32) * 20) 4
-                (4 + mem Ⓓ[ gp ⊖ 920 ⊕ (31 ⊖ clz (mem Ⓓ[ gp ⊖ 1920 ]) 32) * 20 ] ) 4 /\
+                (gp ⊖ 920 ⊕ (31 ⊖ clz (uxTopReadyPriority gp mem) 32) * 20) 4
+                (4 + mem Ⓓ[ gp ⊖ 920 ⊕ (31 ⊖ clz (uxTopReadyPriority gp mem) 32) * 20 ] ) 4 /\
             ~ overlap 32
-                (gp ⊖ 920 ⊕ (31 ⊖ clz (mem Ⓓ[ gp ⊖ 1920 ]) 32) * 20) 4
-                (mem Ⓓ[4 + mem Ⓓ[ gp ⊖ 920 ⊕ (31 ⊖ clz (mem Ⓓ[ gp ⊖ 1920 ]) 32) * 20 ]]) 4)
+                (gp ⊖ 920 ⊕ (31 ⊖ clz (uxTopReadyPriority gp mem) 32) * 20) 4
+                (mem Ⓓ[4 + mem Ⓓ[ gp ⊖ 920 ⊕ (31 ⊖ clz (uxTopReadyPriority gp mem) 32) * 20 ]]) 4)
          ,
   satisfies_all 
     lifted_vTaskSwitchContext                                 (* Provide lifted code *)
@@ -452,13 +429,22 @@ Theorem vTaskSwitchContext_timing:
     vTaskSwitchContext_exit                                   (* Provide exit point *)
   ((x',s')::t).
 Proof using.
+    (* Set up our proof environment *)
     intros.
     apply prove_invs.
     Local Ltac step := time rv_step.
     Local Ltac handle_ex := eexists; eexists; repeat split; try eassumption.
     Local Ltac noverlap_prepare gp sp :=
-        _noverlap_prepare uxSchedulerSuspended pxCurrentTCB 
-            gp_sp_noverlap __global_size vTaskSwitchContext_stack_frame_size 
+        _noverlap_prepare
+            uxSchedulerSuspended pxCurrentTCB __global_size
+             vTaskSwitchContext_stack_frame_size uxSchedulerSuspended 
+             gp_sp_noverlap smem_well_formed pxCurrentTCB_noverlap_static
+             pxCurrentTCB_noverlap_stackframe pxCurrentTCB_noverlap_clz_static
+             clz_noverlap_smem mem_pxCurrentTCB_noverlap_stackframe 
+             mem_pxCurrentTCB_noverlap_static offset_mem_pxCurrentTCB_noverlap_clz
+             clz_noverlap_sframe mem4_pxCurrentTCB_noverlap_stackframe
+             mem4_pxCurrentTCB_noverlap_static uxTopReadyPriority mem4_mem4_noverlap_static
+             mem4_mem4_noverlap_stackframe
             gp sp.
     Local Ltac destruct_noverlaps :=
         match goal with
@@ -492,228 +478,119 @@ Proof using.
         [Preserves920 Cycles]]]]]]]]]]]].
         destruct_noverlaps.
     step. step. step. step. step. step. step. step. step. step.
-    handle_ex. unfold msub. now psimpl.
+    handle_ex.
+        1-10: noverlap_prepare gp sp; memsolve mem gp sp. 
         {
-            noverlap_prepare gp sp; memsolve mem gp sp; auto.
-            all: apply noverlap_symmetry;
-                (apply noverlap_shrink with (sp ⊖ 16) 16;
-                    [ psimpl; lia | apply noverlap_symmetry]);
-                assumption.
-        } {
-            noverlap_prepare gp sp; memsolve mem gp sp; auto.
-            all: try solve [apply noverlap_symmetry;
-                (apply noverlap_shrink with (sp ⊖ 16) 16;
-                    [ psimpl; lia | apply noverlap_symmetry]);
-                assumption].
-        } {
-            unfold pxCurrentTCB_noverlap_static in *.
-            intros. noverlap_prepare gp sp. memsolve mem gp sp; auto.
-        } {
-            unfold pxCurrentTCB_noverlap_stackframe in *.
-            intros. noverlap_prepare gp sp. memsolve mem gp sp; auto.
-        } {
-            unfold pxCurrentTCB_noverlap_clz_static in *.
-            noverlap_prepare gp sp; memsolve mem gp sp; auto.
-        } {
-            unfold clz_noverlap_smem in *. intros.
-            noverlap_prepare gp sp; memsolve mem gp sp; eauto.
-        } {
-            unfold mem_pxCurrentTCB_noverlap_stackframe in *.
-            noverlap_prepare gp sp; memsolve mem gp sp; auto.
-            all: apply noverlap_symmetry, noverlap_shrink with (sp ⊖ 16) 16;
-                [ psimpl; lia |
-                    apply noverlap_symmetry, PCT_NOL_SFRAME ].
-        } {
-            unfold mem_pxCurrentTCB_noverlap_static in *.
-            intros. noverlap_prepare gp sp. memsolve mem gp sp; auto.
-            all: apply noverlap_symmetry, noverlap_shrink with (sp ⊖ 16) 16;
-                [ psimpl; lia |
-                    apply noverlap_symmetry, PCT_NOL_SFRAME ].
-        } {
-            unfold offset_mem_pxCurrentTCB_noverlap_clz. intros.
-            noverlap_prepare gp sp. memsolve mem gp sp; auto.
-            all: apply noverlap_symmetry, noverlap_shrink with (sp ⊖ 16) 16;
-                    [ psimpl; lia |
-                      apply noverlap_symmetry, PCT_NOL_SFRAME ].
-        } {
-            unfold clz_noverlap_sframe. 
-            noverlap_prepare gp sp; memsolve mem gp sp; auto.
-        } {
-            unfold mem4_pxCurrentTCB_noverlap_stackframe. intros.
-            noverlap_prepare gp sp; memsolve mem gp sp; eauto.
-            apply noverlap_symmetry; auto.
-            all: apply noverlap_symmetry, noverlap_shrink with (sp ⊖ 16) 16;
-                [psimpl; lia|auto].
-        } {
-            unfold mem4_pxCurrentTCB_noverlap_static. intros.
-            noverlap_prepare gp sp; memsolve mem gp sp; eauto using noverlap_symmetry.
-            all: apply noverlap_symmetry, noverlap_shrink with (sp ⊖ 16) 16; [
-                psimpl; lia | auto
-            ]; apply noverlap_symmetry, PCT_NOL_SFRAME.
-        } {
             unfold mem4_mem4_noverlap_stackframe.
             noverlap_prepare gp sp; memsolve mem gp sp; eauto using noverlap_symmetry.
-            all: try solve [
-                apply noverlap_symmetry, noverlap_shrink with (sp ⊖ 16) 16;
-                [psimpl;lia|eauto]
-            ].
-            now eapply noverlap_symmetry, MEM4_PCT_NOL_STATIC.
+            now eapply MEM4_PCT_NOL_STATIC.
         } {
             unfold mem4_mem4_noverlap_static. intros.
             noverlap_prepare gp sp; memsolve mem gp sp; eauto using noverlap_symmetry.
-            all: try solve [
-                apply noverlap_symmetry, noverlap_shrink with (sp ⊖ 16) 16;
-                [psimpl;lia|eauto]
-            ].
-            now eapply noverlap_symmetry, MEM4_PCT_NOL_STATIC.
+            now eapply MEM4_PCT_NOL_STATIC.
         } {
             noverlap_prepare gp sp; memsolve mem gp sp; eauto using noverlap_symmetry.
-            all: apply noverlap_symmetry, noverlap_shrink with (sp ⊖ 16) 16;
-                [psimpl;lia|eauto].
         } {
             noverlap_prepare gp sp; memsolve mem gp sp; eauto using noverlap_symmetry.
-            all: try solve [apply noverlap_symmetry, noverlap_shrink with (sp ⊖ 16) 16;
-                [psimpl;lia|eauto]].
-            now eapply noverlap_symmetry, MEM4_PCT_NOL_STATIC.
+            now eapply MEM4_PCT_NOL_STATIC.
         } {
-            unfold uxTopReadyPriority. 
             noverlap_prepare gp sp; memsolve mem gp sp; auto.
         } {
             noverlap_prepare gp sp.
             repeat rewrite <- getmem_mod_l with (a := _ + _).
             rewrite getmem_mod_l.
-            replace (clz _ 32) with (clz (mem Ⓓ[gp ⊖ 1920]) 32) by memsolve mem gp sp.
+            replace (clz _ 32) with (clz (uxTopReadyPriority gp mem) 32) by memsolve mem gp sp.
             replace ((mem [Ⓓgp ⊖ 1932 := 0 ] [Ⓓsp ⊖ 8 := n ] [Ⓓsp ⊖ 4 := n0 ])
-                Ⓓ[ gp ⊖ 920 ⊕ (31 ⊖ clz (mem Ⓓ[ gp ⊖ 1920 ]) 32) * 20 ]) with
-                (mem Ⓓ[ gp ⊖ 920 ⊕ (31 ⊖ clz (mem Ⓓ[ gp ⊖ 1920 ]) 32) * 20 ]); cycle 1.
-                memsolve mem gp sp. eauto using noverlap_symmetry.
-                1-2: try solve [apply noverlap_symmetry, noverlap_shrink with (sp ⊖ 16) 16;
-                    [psimpl; lia|auto]].
+                Ⓓ[ gp ⊖ 920 ⊕ (31 ⊖ clz (uxTopReadyPriority gp mem) 32) * 20 ]) with
+                (mem Ⓓ[ gp ⊖ 920 ⊕ (31 ⊖ clz (uxTopReadyPriority gp mem) 32) * 20 ]); cycle 1.
+                memsolve mem gp sp.
             rewrite getmem_mod_l.
             replace ((mem [Ⓓgp ⊖ 1932 := 0 ] [Ⓓsp ⊖ 8 := n ] [Ⓓsp ⊖ 4 := n0 ])
-                Ⓓ[ 4 + mem Ⓓ[ gp ⊖ 920 ⊕ (31 ⊖ clz (mem Ⓓ[ gp ⊖ 1920 ]) 32) * 20 ] ]) with
-                (mem Ⓓ[ 4 + mem Ⓓ[ gp ⊖ 920 ⊕ (31 ⊖ clz (mem Ⓓ[ gp ⊖ 1920 ]) 32) * 20 ] ]); cycle 1.
-                memsolve mem gp sp. apply noverlap_symmetry.
-                    now eapply MEM4_PCT_NOL_STATIC.
-                1-2: try solve [apply noverlap_symmetry, noverlap_shrink with (sp ⊖ 16) 16;
-                    [psimpl; lia|auto]].
-            memsolve mem gp sp; eauto using noverlap_symmetry.
-            now repeat rewrite getmem_mod_l; rewrite Preserves920.
-            all: try solve [apply noverlap_symmetry, noverlap_shrink with (sp ⊖ 16) 16;
-                [psimpl; lia|auto]].
-            all: apply noverlap_symmetry; rewrite<- getmem_mod_l. 
+                Ⓓ[ 4 + mem Ⓓ[ gp ⊖ 920 ⊕ (31 ⊖ clz (uxTopReadyPriority gp mem) 32) * 20 ] ]) with
+                (mem Ⓓ[ 4 + mem Ⓓ[ gp ⊖ 920 ⊕ (31 ⊖ clz (uxTopReadyPriority gp mem) 32) * 20 ] ]); cycle 1.
+                memsolve mem gp sp. now eapply MEM4_PCT_NOL_STATIC.
+            memsolve mem gp sp.
+            unfold uxTopReadyPriority. now repeat rewrite getmem_mod_l; rewrite Preserves920.
+            all: rewrite <- getmem_mod_l. 
                 now eapply MEM4_PCT_NOL_STATIC.
             all: apply noverlap_shrink with (sp ⊖ 16) 16;
                 [psimpl; lia|auto].
         }
         hammer. rewrite A4, BC, Cycles. lia.
     step. step.
-        unfold timing_postcondition.
+        unfold time_of_vTaskSwitchContext.
         rewrite BC.
         hammer. rewrite A4, BC, Cycles. lia.
 
     (* 0x800013c8 *)
-    destruct PRE as [mem [MEM [GP [SP [A5 [A2 [A4 [NOVERLAPS [MEM4_MEM4_NOL_SFRAME
+    destruct PRE as [mem [MEM [GP [NOVERLAPS [MEM4_MEM4_NOL_SFRAME
         [MEM4_MEM4_NOL_STATIC [MEM4_920 [MEM4_MEM4_920 [PreservesPriority 
-        [Preserves920 [BR0 Cycles]]]]]]]]]]]]]]].
-        destruct_noverlaps.
+        [Preserves920 [Suspended Cycles]]]]]]]]]]]. destruct_noverlaps.
     step.
         step. step. step. step. step. step. step. step. step. step.
         exact I. (* Infinite loop, stack overflow detected *)
     step. handle_ex.
-        now apply Bool.negb_false_iff in BC.
-        change ((678490 << 12) + 1445) with 0xa5a5a5a5 in *.
-        hammer. rewrite A2, A4, BC, Cycles. lia.
+        hammer. rewrite Hsv, Hsv0, BC, Cycles. lia.
 
     (* 0x800013d0 *)
-    destruct PRE as [mem [MEM [GP [SP [A2 [A3 [A5 [NOVERLAPS [MEM4_MEM4_NOL_SFRAME
+    destruct PRE as [mem [MEM [GP [NOVERLAPS [MEM4_MEM4_NOL_SFRAME
         [MEM4_MEM4_NOL_STATIC [MEM4_920 [MEM4_MEM4_920 [PreservesPriority [Preserves920 
-        [NotSuspended [Br Cycles]]]]]]]]]]]]]]]].
+        [NotSuspended Cycles]]]]]]]]]]].
     destruct_noverlaps.
     step.
         step. step. step. step. step. step. step. step. step. step.
         exact I. (* Infinite loop, stack overflow detected *)
     step. handle_ex.
-        now apply Bool.negb_false_iff in BC.
-        hammer. rewrite A2, A3, Cycles, BC. lia.
+        hammer. rewrite Hsv, Hsv0, Cycles, BC. lia.
 
     (* 0x800013d8 *)
-    destruct PRE as [mem [MEM [GP [SP [A3 [A4 [A5 [NOVERLAPS [MEM4_MEM4_NOL_SFRAME
+    destruct PRE as [mem [MEM [GP [NOVERLAPS [MEM4_MEM4_NOL_SFRAME
         [MEM4_MEM4_NOL_STATIC [MEM4_920 [MEM4_MEM4_920 [PreservesPriority [Preserves920 
-        [B1 [B2 [NotSuspended Cycles]]]]]]]]]]]]]]]]]. destruct_noverlaps.
+        [NotSuspended Cycles]]]]]]]]]]]. destruct_noverlaps.
     step.
         step. step. step. step. step. step. step. step. step. step.
         exact I. (* Infinite loop, stack overflow detected *)
     step.
         handle_ex.
-        now apply Bool.negb_false_iff in BC.
-        hammer. rewrite A3, A4, BC, Cycles. lia.
+        hammer. rewrite Hsv, Hsv0, BC, Cycles. lia.
 
     (* 0x800013e0 *)
-    destruct PRE as [mem [MEM [GP [SP [A3 [A4 [A5 [NOVERLAPS [MEM4_MEM4_NOL_SFRAME 
+    destruct PRE as [mem [MEM [GP [NOVERLAPS [MEM4_MEM4_NOL_SFRAME 
         [MEM4_MEM4_NOL_STATIC [MEM4_920 [MEM4_MEM4_920 [PreservesPriority 
-        [Preserves920 [B1 [B2 [B3 [NotSuspended Cycles]]]]]]]]]]]]]]]]]]. destruct_noverlaps.
+        [Preserves920 [NotSuspended Cycles]]]]]]]]]]]. destruct_noverlaps.
     step. step. step. step. step. step. step. step. step. step. step.
     step. step. step. step.
         handle_ex.
+        Require Import memsolve.
+            1-15: try solve [noverlap_prepare gp sp; memsolve mem gp sp].
         {
             unfold uxTopReadyPriority.
             noverlap_prepare gp sp.
             replace (clz
             ((mem [Ⓓgp ⊖ 920 ⊕ (31 ⊖ clz (mem Ⓓ[ gp ⊖ 1920 ]) 32) * 20
               := mem
-                 Ⓓ[ 4 + mem Ⓓ[ gp ⊖ 920 ⊕ (31 ⊖ clz (mem Ⓓ[ gp ⊖ 1920 ]) 32) * 20 ]
-                 ] ]) Ⓓ[ gp ⊖ 1920 ]) 32) with 
-                (clz (mem Ⓓ[ gp ⊖ 1920 ]) 32); cycle 1. {
-                f_equal. memsolve mem gp sp; auto.
-            } psimpl. reflexivity.
+                 Ⓓ[ 4 +
+                    mem Ⓓ[ gp ⊖ 920 ⊕ (31 ⊖ clz (mem Ⓓ[ gp ⊖ 1920 ]) 32) * 20
+                    ] ] ]) Ⓓ[ gp ⊖ 1920 ]) 32) with 
+                (clz (mem Ⓓ[ gp ⊖ 1920 ]) 32) by
+                (f_equal; memsolve mem gp sp; auto).
+            unfold msub at 4. now psimpl.
         } {
-            unfold addr_pxReadyTasksLists, uxTopReadyPriority.
-            noverlap_prepare gp sp; memsolve mem gp sp; auto.
-        } {
-            unfold uxTopReadyPriority.
-            noverlap_prepare gp sp; memsolve mem gp sp; auto.
-        }
-        now unfold addr_pxReadyTasksLists, msub; psimpl.
-        {
-            unfold uxTopReadyPriority.
-            noverlap_prepare gp sp; memsolve mem gp sp; auto. f_equal.
+            noverlap_prepare gp sp; memsolve mem gp sp. unfold addr_pxReadyTasksLists.
             unfold msub; psimpl; simpl (2^32 - _ mod _).
                 now rewrite N.add_comm, N.add_assoc,
                     (N.add_comm _ gp), getmem_mod_l.
         } {
-            unfold pxCurrentTCB_noverlap_static. intros.
-            noverlap_prepare gp sp; memsolve mem gp sp; auto.
-        } {
-            unfold pxCurrentTCB_noverlap_stackframe.
-            noverlap_prepare gp sp; memsolve mem gp sp; auto.
-        } {
-            unfold pxCurrentTCB_noverlap_clz_static.
-            noverlap_prepare gp sp; memsolve mem gp sp; auto.
-        } {
-            unfold clz_noverlap_smem. intros.
             noverlap_prepare gp sp.
             replace ((mem [Ⓓgp ⊖ 920 ⊕ (31 ⊖ clz (mem Ⓓ[ gp ⊖ 1920 ]) 32) * 20
             := mem
                Ⓓ[ 4 +
                   mem Ⓓ[ gp ⊖ 920 ⊕ (31 ⊖ clz (mem Ⓓ[ gp ⊖ 1920 ]) 32) * 20 ]
-               ] ]) Ⓓ[ gp ⊖ 1920 ]) with (mem Ⓓ[gp ⊖ 1920]) by
+               ] ]) Ⓓ[ gp ⊖ 1920 ]) with (mem Ⓓ[ gp ⊖ 1920 ]) by
                (rewrite getmem_noverlap; auto).
-           eapply CLZ_NOL_STATIC; eassumption.
+            rewrite N.add_comm.
+            now unfold msub; psimpl; simpl (2^32 - _ mod _).
         } {
-            unfold mem_pxCurrentTCB_noverlap_stackframe.
-            noverlap_prepare gp sp; memsolve mem gp sp; auto.
-        } {
-            unfold mem_pxCurrentTCB_noverlap_static. intros.
-            noverlap_prepare gp sp; memsolve mem gp sp; auto.
-        } {
-            unfold offset_mem_pxCurrentTCB_noverlap_clz. intros.
-            noverlap_prepare gp sp; memsolve mem gp sp; auto.
-        } {
-            unfold clz_noverlap_sframe.
-            noverlap_prepare gp sp; memsolve mem gp sp; auto.
-        } {
-            unfold mem4_pxCurrentTCB_noverlap_stackframe.
             noverlap_prepare gp sp.
             replace (clz ((mem [Ⓓ_ := _ ]) Ⓓ[ gp ⊖ 1920 ]) 32) 
                 with (clz (mem Ⓓ[ gp ⊖ 1920 ]) 32) by
@@ -722,7 +599,6 @@ Proof using.
             rewrite <- getmem_mod_l with (a := gp ⊖ _ + _).
             eapply MEM4_MEM4_NOL_SFRAME.
         } {
-            unfold mem4_pxCurrentTCB_noverlap_static. intros.
             noverlap_prepare gp sp.
             replace (clz ((mem [Ⓓ_ := _ ]) Ⓓ[ gp ⊖ 1920 ]) 32) 
                 with (clz (mem Ⓓ[ gp ⊖ 1920 ]) 32) by
@@ -730,19 +606,15 @@ Proof using.
             psimpl.
             rewrite <- getmem_mod_l with (a := gp ⊖ _ + _).
             eapply MEM4_MEM4_NOL_STATIC; eassumption.
-        } {
-            unfold uxTopReadyPriority.
-            noverlap_prepare gp sp; memsolve mem gp sp; auto.
-        } { noverlap_prepare gp sp.
+        } { 
+            noverlap_prepare gp sp.
             replace (clz ((mem [Ⓓ_ := _ ]) Ⓓ[ gp ⊖ 1920 ]) 32) 
                 with (clz (mem Ⓓ[ gp ⊖ 1920 ]) 32) by
                 (f_equal; rewrite getmem_noverlap; auto).
             psimpl.
             now rewrite Preserves920.
-        } { 
-            noverlap_prepare gp sp; memsolve mem gp sp; auto.
         }
-        hammer. rewrite A4, A5, BC, Cycles. psimpl.
+        hammer. rewrite Hsv, Hsv0, BC, Cycles. psimpl.
         noverlap_prepare gp sp.
         replace (clz ((mem [Ⓓ_ := _ ]) Ⓓ[ gp ⊖ 1920 ]) 32) 
                 with (clz (mem Ⓓ[ gp ⊖ 1920 ]) 32) by
@@ -751,29 +623,27 @@ Proof using.
     (* Inside vApplicationStackOverflowHook *)
     step. step. step. step. step. step. step. step. step. step. exact I.
 
-    destruct PRE as [mem [MEM [GP [SP [A1 [A2 [A3 [A4 [A5 [NOVERLAPS
-        [PreservesPriority [Preserves920 [NotSuspended [B1 Cycles]]]]]]]]]]]]]].
+    destruct PRE as [mem [MEM [GP [A1 [A2 [A5 [NOVERLAPS
+        [PreservesPriority [Preserves920 [NotSuspended Cycles]]]]]]]]]].
     destruct_noverlaps.
     step. step. step. step. step. step. step. step. step. step. step.
-    unfold timing_postcondition.
-    (* unfold uxTopReadyPriority. noverlap_prepare gp sp. *)
+    unfold time_of_vTaskSwitchContext.
+    rewrite getmem_mod_l with (m := base_mem) (a := gp ⊖ _ + _).
+    rewrite <- Preserves920, <- PreservesPriority.
+    apply Bool.negb_true_iff in BC.
     replace (4 + (gp ⊖ 924) ⊕ (31 ⊖ clz (uxTopReadyPriority gp mem) 32) * 20) with
         ((gp ⊖ 920) ⊕ (31 ⊖ clz (uxTopReadyPriority gp mem) 32) * 20) in BC by
         (unfold msub; now psimpl).
-    rewrite <- getmem_mod_l with (m := base_mem) (a := gp ⊖ _ + _) in Preserves920.
-    unfold uxTopReadyPriority in *.
-    rewrite <- Preserves920, <- PreservesPriority.
-    apply Bool.negb_true_iff in BC.
     rewrite getmem_mod_l in BC. rewrite BC, NotSuspended.
     hammer. rewrite A1, A5.
     replace (4 + _ ⊕ _) with ((gp ⊖ 920) ⊕ (31 ⊖ clz (mem Ⓓ[ gp ⊖ 1920 ]) 32) * 20)
         by (unfold msub; now psimpl).
+    unfold uxTopReadyPriority in *.
     rewrite getmem_mod_l, BC, Cycles.
-    cbn [negb]. psimpl. unfold msub in PreservesPriority.
-    psimpl in PreservesPriority. rewrite PreservesPriority. lia.
+    cbn [negb]. psimpl. lia.
 
     step. step. step. step. step. step. step. step. step. step. step. step.
-    unfold timing_postcondition.
+    unfold time_of_vTaskSwitchContext.
     apply Bool.negb_false_iff in BC.
     replace (4 + _ ⊕ _) with ((gp ⊖ 920) ⊕ (31 ⊖ clz (mem Ⓓ[ gp ⊖ 1920 ]) 32) * 20)
         in BC by (unfold msub; now psimpl).
@@ -785,8 +655,7 @@ Proof using.
     replace (4 + _ ⊕ _) with ((gp ⊖ 920) ⊕ (31 ⊖ clz (mem Ⓓ[ gp ⊖ 1920 ]) 32) * 20)
         by (unfold msub; now psimpl).
     unfold uxTopReadyPriority in *. rewrite getmem_mod_l, BC, Cycles.
-    cbn [negb]. psimpl. unfold msub in PreservesPriority.
-    psimpl in PreservesPriority. rewrite PreservesPriority. lia.
+    cbn [negb]. psimpl. lia.
 
     step. exact I.
 Qed.
